finish reverting to simpler stack representation

parser/Parser.v
@@ -33,11 +33,11 @@ Module ParserFn (Import D : Defs.T).
   | StepError  : parse_error -> step_result.
 
   Lemma lhss_invar_eqs :
-    forall rm sk x pre vs suf y suf' frs,
-      stack_lhss_from_keyset rm sk
-      -> sk = (Fr x pre vs suf, frs)
-      -> suf = NT y :: suf'
-      -> stack_lhss_from_keyset rm (Fr x pre vs (NT y :: suf'), frs).
+    forall rm sk pre vs suf x suf' frs,
+      stack_pushes_from_keyset rm sk
+      -> sk = (Fr pre vs suf, frs)
+      -> suf = NT x :: suf'
+      -> stack_pushes_from_keyset rm (Fr pre vs (NT x :: suf'), frs).
   Proof.
     intros; subst; auto.
   Qed.
@@ -74,45 +74,46 @@ Module ParserFn (Import D : Defs.T).
              (un : bool) 
              (ca : cache)
              (hc : cache_stores_target_results rm cm ca)
-             (hk : stack_lhss_from_keyset rm sk) : step_result :=
+             (hk : stack_pushes_from_keyset rm sk) : step_result :=
     match sk as sk' return sk = sk' -> _ with
-    | (Fr x pre vs suf, frs) =>
+    | (Fr pre vs suf, frs) =>
       fun hsk =>
         match suf as suf' return suf = suf' -> _ with
         (* no more symbols to process in current frame *)
         | [] =>
           fun _ =>
             match frs with
-            (* empty stacks --> terminate *)
+            (* empty stack --> terminate *)
             | [] => 
               match ts with
               | [] =>
                 match pre, vs with
-                | [NT y], (v, tt) => StepAccept y v
+                | [NT x], (v, tt) => StepAccept x v
                 | _, _ => StepError InvalidState
                 end
               | t :: _ => StepReject (emptyStackMsg t)
               end
-            (* nonempty stacks --> return to caller frames *)
-            | Fr x_cr pre_cr vs_cr suf_cr :: frs' =>
+            (* nonempty stack --> return to caller frame *)
+            | Fr pre_cr vs_cr (NT x :: suf_cr) :: frs' =>
               let pre' := rev pre in
               let vs'  := revTuple pre vs in
               match findPredicateAndAction (x, pre') gr hw with
               (* check predicate and reduce *)
               | Some (Some p, f) =>
                 if p vs' then
-                  let sk' := (Fr x_cr (NT x :: pre_cr) (f vs', vs_cr) suf_cr, frs')
+                  let sk' := (Fr (NT x :: pre_cr) (f vs', vs_cr) suf_cr, frs')
                   in  StepK sk' ts (NtSet.remove x vi) un ca
                 else
                   StepReject "some failed predicate message here"
               (* reduce *)
               | Some (None, f) =>
-                let sk' := (Fr x_cr (NT x :: pre_cr) (f vs', vs_cr) suf_cr, frs')
+                let sk' := (Fr (NT x :: pre_cr) (f vs', vs_cr) suf_cr, frs')
                 in  StepK sk' ts (NtSet.remove x vi) un ca
               (* impossible case *)
               | None =>
                 StepError InvalidState
               end
+            | _ => StepError InvalidState
             end
         (* terminal case --> consume a token *)
         | T a :: suf' =>
@@ -121,32 +122,32 @@ Module ParserFn (Import D : Defs.T).
             | []             => StepReject (emptyInputMsg a)
             | @existT _ _ a' v :: ts' =>
               if t_eq_dec a' a then
-                let sk' := (Fr x (T a' :: pre) (v, vs) suf', frs)
+                let sk' := (Fr (T a' :: pre) (v, vs) suf', frs)
                 in  StepK sk' ts' NtSet.empty un ca
               else
                 StepReject (mismatchMsg a (@existT _ _ a' v))
             end
         (* nonterminal case --> push a frame onto the stack *)
-        | NT y :: suf' =>
+        | NT x :: suf' =>
           fun hsuf =>
-            if NtSet.mem y vi then
+            if NtSet.mem x vi then
               (* Unreachable for a left-recursive grammar *)
-              match NM.find y rm with
-              | Some _ => StepError (LeftRecursion y) 
-              | None   => StepReject (notFoundMsg y)
+              match NM.find x rm with
+              | Some _ => StepError (LeftRecursion x) 
+              | None   => StepReject (notFoundMsg x)
               end
             else
-              match adaptivePredict gr hw rm cm x pre vs y suf' frs ts ca hc
-                                    (lhss_invar_eqs _ _ _ _ _ _ _ _ _ hk hsk hsuf)
+              match adaptivePredict gr hw rm cm pre vs x suf' frs ts ca hc
+                                    (lhss_invar_eqs _ _ _ _ _ _ _ _ hk hsk hsuf)
               with
               | (PredSucc rhs, ca') =>
-                let sk' := (Fr y [] tt rhs, Fr x pre vs suf' :: frs) in
-                StepK sk' ts (NtSet.add y vi) un ca'
+                let sk' := (Fr [] tt rhs, Fr pre vs (NT x :: suf') :: frs) in
+                StepK sk' ts (NtSet.add x vi) un ca'
               | (PredAmbig rhs, ca') =>
-                let sk' := (Fr y [] tt rhs, Fr x pre vs suf' :: frs) in
-                StepK sk' ts (NtSet.add y vi) false ca'
+                let sk' := (Fr [] tt rhs, Fr pre vs (NT x :: suf') :: frs) in
+                StepK sk' ts (NtSet.add x vi) false ca'
               | (PredReject, _)  =>
-                StepReject (failedPredictionMsg y ts)
+                StepReject (failedPredictionMsg x ts)
               | (PredError e, _) =>
                 StepError (PredictionError e) 
               end
@@ -154,27 +155,27 @@ Module ParserFn (Import D : Defs.T).
     end eq_refl.
 
   Lemma step_StepAccept_facts :
-    forall gr hw rm cm sk ts vi un ca hc hk y v,
-      step gr hw rm cm sk ts vi un ca hc hk = StepAccept y v
+    forall gr hw rm cm sk ts vi un ca hc hk x v,
+      step gr hw rm cm sk ts vi un ca hc hk = StepAccept x v
       -> ts = []
-         /\ exists x, sk = (Fr x [NT y] (v, tt) [], []).
+         /\ sk = (Fr [NT x] (v, tt) [], []).
   Proof.
     intros gr hw rm cm sk ts vi un ca hc hk y v hs.
     unfold step in hs; dms; tc.
-    inv hs; eauto.
+    inv hs; auto. 
   Qed.
 
   Lemma step_LeftRecursion_facts :
-    forall gr hw rm cm sk ts vi un ca hc hk y,
-      step gr hw rm cm sk ts vi un ca hc hk = StepError (LeftRecursion y)
-      -> NtSet.In y vi
-         /\ (exists yss, NM.find y rm = Some yss)
-         /\ (exists x pre vs suf frs,
-             sk = (Fr x pre vs (NT y :: suf), frs)). 
+    forall gr hw rm cm sk ts vi un ca hc hk x,
+      step gr hw rm cm sk ts vi un ca hc hk = StepError (LeftRecursion x)
+      -> NtSet.In x vi
+         /\ (exists yss, NM.find x rm = Some yss)
+         /\ (exists pre vs suf frs,
+             sk = (Fr pre vs (NT x :: suf), frs)). 
   Proof.
-    intros gr hw cm rm sk ts vi un ca hc hk y hs.
+    intros gr hw cm rm sk ts vi un ca hc hk x hs.
     unfold step in hs; repeat dmeq h; tc; inv hs; sis;
-      repeat split; eauto 6.
+      repeat split; eauto.
     apply NF.mem_iff; auto.
   Qed.
 
@@ -189,21 +190,21 @@ Module ParserFn (Import D : Defs.T).
     - eapply adaptivePredict_ambig_preserves_cache_invar; eauto.
   Defined.
 
-  Lemma step_preserves_lhss_invar :
+  Lemma step_preserves_pki :
     forall gr hw rm cm sk sk' ts ts' vi vi' un un' ca ca' hc hk,
       rhs_map_correct rm gr
       -> step gr hw rm cm sk ts vi un ca hc hk = StepK sk' ts' vi' un' ca'
-      -> stack_lhss_from_keyset rm sk'.
+      -> stack_pushes_from_keyset rm sk'.
   Proof.
     intros gr hw rm cm sk sk' ts ts' vi vi' un un' ca ca' hc hk hr hs.
     unfold step in hs; dmeqs H; tc; inv hs; red; red in hk; sis.
-    - eapply sll_return_preserves_keyset_invar; eauto.
-    - eapply sll_return_preserves_keyset_invar; eauto.
-    - eapply sll_consume_preserves_keyset_invar; eauto.
-    - eapply sll_push_preserves_keyset_invar; eauto.
+    - eapply return_preserves_keyset_invar; eauto.
+    - eapply return_preserves_keyset_invar; eauto.
+    - eapply consume_preserves_keyset_invar; eauto.
+    - eapply push_preserves_keyset_invar; eauto.
       eapply rhssFor_keySet.
       eapply adaptivePredict_succ_in_rhssFor; eauto.
-    - eapply sll_push_preserves_keyset_invar; eauto.
+    - eapply push_preserves_keyset_invar; eauto.
       eapply rhssFor_keySet.
       (* lemma relating SLL and LL prediction *)
       (*
@@ -217,63 +218,63 @@ Module ParserFn (Import D : Defs.T).
       eapply llPredict_ambig_in_rhssFor; eauto.
   Qed.
 
-  Definition meas (rm : rhs_map)
-                  (sk : parser_stack)
-                  (ts : list token)
-                  (vi :  NtSet.t) : nat * nat * nat :=
-    let (stkScore, stkHeight) := ss_meas rm vi (sllify sk)
+  Definition parser_meas
+             (rm : rhs_map)
+             (sk : parser_stack)
+             (ts : list token)
+             (vi :  NtSet.t) : nat * nat * nat :=
+    let (stkScore, stkHeight) := meas rm vi (stackSuffixes sk)
     in  (List.length ts, stkScore, stkHeight).
 
-  Lemma meas_lt_after_return :
-    forall rm ce cr cr' x y pre pre' pre'' vs vs' vs'' suf frs ts vi,
-      ce     = Fr y pre' vs' []
-      -> cr  = Fr x pre vs suf
-      -> cr' = Fr x pre'' vs'' suf
-      -> stack_lhss_from_keyset rm (ce, cr :: frs)
-      -> lex_nat_triple (meas rm (cr', frs) ts (NtSet.remove y vi))
-                        (meas rm (ce, cr :: frs) ts vi).
+  Lemma parser_meas_lt_after_return :
+    forall rm ce cr cr' pre pre' pre'' vs vs' vs'' x suf frs ts vi,
+      ce     = Fr pre' vs' []
+      -> cr  = Fr pre vs (NT x :: suf)
+      -> cr' = Fr pre'' vs'' suf
+      -> stack_pushes_from_keyset rm (ce, cr :: frs)
+      -> lex_nat_triple (parser_meas rm (cr', frs) ts (NtSet.remove x vi))
+                        (parser_meas rm (ce, cr :: frs) ts vi).
   Proof.
-    intros ? ? ? ? ? ? ? ? ? ? ? ? ? ? ? ? ? ? ? hk; subst; unfold meas.
+    intros ? ? ? ? ? ? ? ? ? ? ? ? ? ? ? ? ? ? hk; subst; unfold meas.
     red in hk.
-    eapply ss_meas_lt_after_return with (vi := vi) in hk; sis; eauto.
+    eapply meas_lt_after_return with (vi := vi) in hk; sis; eauto.
     inversion hk as [ ? ? ? ? hl | ? ? ? hl heq heq']; subst; clear hk.
     - apply triple_snd_lt; auto.
-    - rewrite heq'.
+    - unfold parser_meas; sis; rewrite heq'.
       apply triple_thd_lt; auto.
   Defined.
 
-  Lemma meas_lt_after_push :
-    forall rm cr cr' ce x pre vs y suf rhs frs ts vi,
-      cr = Fr x pre vs (NT y :: suf)
-      -> cr' = Fr x pre vs suf
-      -> ce = Fr y [] tt rhs
-      -> In rhs (rhssFor y rm)
-      -> NtSet.mem y vi = false 
-      -> lex_nat_triple (meas rm (ce, cr' :: frs) ts (NtSet.add y vi))
-                        (meas rm (cr, frs) ts vi).
+  Lemma parser_meas_lt_after_push :
+    forall rm cr ce pre vs x suf rhs frs ts vi,
+      cr = Fr pre vs (NT x :: suf)
+      -> ce = Fr [] tt rhs
+      -> In rhs (rhssFor x rm)
+      -> NtSet.mem x vi = false 
+      -> lex_nat_triple (parser_meas rm (ce, cr :: frs) ts (NtSet.add x vi))
+                        (parser_meas rm (cr, frs) ts vi).
   Proof.
-    intros ? ? ? ? ? ? ? ? ? ? ? ? ? ? ? ? hi hm; subst.
+    intros ? ? ? ? ? ? ? ? ? ? ? ? ? hi hm; subst.
     apply triple_snd_lt.
-    apply stackScore_lt_after_push; sis; auto.
+    eapply stackScore_lt_after_push; sis; auto.
     - eapply rhssFor_keySet; eauto.
     - apply NF.not_mem_iff in hm; auto.
     - eapply rhssFor_allRhss; eauto.
   Defined.
   
-  Lemma step_meas_lt :
+  Lemma step_parser_meas_lt :
     forall gr hw rm cm sk sk' ts ts' vi vi' un un' ca ca' hc hk,
       step gr hw rm cm sk ts vi un ca hc hk = StepK sk' ts' vi' un' ca'
-      -> lex_nat_triple (meas rm sk' ts' vi') (meas rm sk ts vi).
+      -> lex_nat_triple (parser_meas rm sk' ts' vi') (parser_meas rm sk ts vi).
   Proof.
     intros gr hw rm cm sk sk' ts ts' vi vi' un un' ca ca' hc hk hs; unfold step in hs.
-    destruct sk as ([x pre vs suf], frs).
+    destruct sk as ([pre vs suf], frs).
     dmeqs H; tc; inv hs.
-    - eapply meas_lt_after_return with (pre'' := NT x :: _); eauto.
-    - eapply meas_lt_after_return with (pre'' := NT x :: _); eauto.
+    - eapply parser_meas_lt_after_return with (pre'' := NT _ :: _); eauto.
+    - eapply parser_meas_lt_after_return with (pre'' := NT _ :: _); eauto.
     - apply triple_fst_lt; auto.
-    - eapply meas_lt_after_push; eauto.
+    - eapply parser_meas_lt_after_push; eauto.
       eapply adaptivePredict_succ_in_rhssFor; eauto.
-    - eapply meas_lt_after_push; eauto.
+    - eapply parser_meas_lt_after_push; eauto.
       (* lemma relating SLL and LL prediction *)
       (*
       eapply llPredict_ambig_in_rhssFor; eauto.
@@ -288,12 +289,12 @@ Module ParserFn (Import D : Defs.T).
 
   Lemma StepK_result_acc :
     forall gr hw rm cm sk sk' ts ts' vi vi' un un' ca ca'
-           hc hk (a : Acc lex_nat_triple (meas rm sk ts vi)),
+           hc hk (a : Acc lex_nat_triple (parser_meas rm sk ts vi)),
       step gr hw rm cm sk ts vi un ca hc hk = StepK sk' ts' vi' un' ca'
-      -> Acc lex_nat_triple (meas rm sk' ts' vi').
+      -> Acc lex_nat_triple (parser_meas rm sk' ts' vi').
   Proof.
     intros; eapply Acc_inv; eauto.
-    eapply step_meas_lt; eauto.
+    eapply step_parser_meas_lt; eauto.
   Defined.
 
   Inductive parse_result : Type :=
@@ -323,8 +324,8 @@ Module ParserFn (Import D : Defs.T).
            (un : bool)
            (ca : cache)
            (hc : cache_stores_target_results rm cm ca)
-           (hk : stack_lhss_from_keyset rm sk)
-           (ha : Acc lex_nat_triple (meas rm sk ts vi))
+           (hk : stack_pushes_from_keyset rm sk)
+           (ha : Acc lex_nat_triple (parser_meas rm sk ts vi))
            {struct ha} : parse_result :=
     match step gr hw rm cm sk ts vi un ca hc hk as res return step gr hw rm cm sk ts vi un ca hc hk = res -> _ with
     | StepAccept x v            => fun _  => if un then Accept x v else Ambig x v
@@ -333,7 +334,7 @@ Module ParserFn (Import D : Defs.T).
     | StepK sk' ts' vi' un' ca' =>
       fun hs => multistep gr hw rm hr cm sk' ts' vi' un' ca'
                           (step_preserves_cache_invar _ _ _ _ _ _ _ _ _ _ _ _ _ _ hc hk hs)
-                          (step_preserves_lhss_invar _ _ _ _ _ _ _ _ _ _ _ _ _ _ hc hk hr hs)
+                          (step_preserves_pki _ _ _ _ _ _ _ _ _ _ _ _ _ _ hc hk hr hs)
                           (StepK_result_acc _ _ _ _ _ _ _ _ _ _ _ _ _ _ hc hk ha hs)
     end eq_refl.
 
@@ -347,7 +348,7 @@ Module ParserFn (Import D : Defs.T).
       | StepK sk' ts' vi' un' ca' =>
         fun hs => multistep gr hw rm hr cm sk' ts' vi' un' ca'
                             (step_preserves_cache_invar _ _ _ _ _ _ _ _ _ _ _ _ _ _ hc hk hs)
-                            (step_preserves_lhss_invar _ _ _ _ _ _ _ _ _ _ _ _ _ _ hc hk hr hs)
+                            (step_preserves_pki _ _ _ _ _ _ _ _ _ _ _ _ _ _ hc hk hr hs)
                             (StepK_result_acc _ _ _ _ _ _ _ _ _ _ _ _ _ _ hc hk ha hs)
       end eq_refl.
   Proof.
@@ -366,8 +367,8 @@ Module ParserFn (Import D : Defs.T).
            (un  : bool)
            (ca  : cache)
            (hc  : cache_stores_target_results rm cm ca)
-           (hk  : stack_lhss_from_keyset rm sk)
-           (ha  : Acc lex_nat_triple (meas rm sk ts vi))
+           (hk  : stack_pushes_from_keyset rm sk)
+           (ha  : Acc lex_nat_triple (parser_meas rm sk ts vi))
            (sr  : step_result)
            (pr  : parse_result)
            (heq : step gr hw rm cm sk ts vi un ca hc hk = sr),
@@ -378,7 +379,7 @@ Module ParserFn (Import D : Defs.T).
       | StepK sk' ts' vi' un' ca' =>
         fun hs => multistep gr hw rm hr cm sk' ts' vi' un' ca'
                             (step_preserves_cache_invar _ _ _ _ _ _ _ _ _ _ _ _ _ _ hc hk hs)
-                            (step_preserves_lhss_invar _ _ _ _ _ _ _ _ _ _ _ _ _ _ hc hk hr hs)
+                            (step_preserves_pki _ _ _ _ _ _ _ _ _ _ _ _ _ _ hc hk hr hs)
                             (StepK_result_acc _ _ _ _ _ _ _ _ _ _ _ _ _ _ hc hk ha hs)
       end heq = pr
       -> match pr with
@@ -417,8 +418,8 @@ Module ParserFn (Import D : Defs.T).
            (un  : bool)
            (ca  : cache)
            (hc  : cache_stores_target_results rm cm ca)
-           (hk  : stack_lhss_from_keyset rm sk)
-           (ha  : Acc lex_nat_triple (meas rm sk ts vi))
+           (hk  : stack_pushes_from_keyset rm sk)
+           (ha  : Acc lex_nat_triple (parser_meas rm sk ts vi))
            (pr  : parse_result),
       multistep gr hw rm hr cm sk ts vi un ca hc hk ha = pr
       -> match pr with
@@ -455,7 +456,7 @@ Module ParserFn (Import D : Defs.T).
 
   Lemma push_invar_starts_true :
     forall rm x,
-      stack_lhss_from_keyset rm (Fr x [] tt [NT x], []). 
+      stack_pushes_from_keyset rm (Fr [] tt [NT x], []). 
   Proof.
     intros rm x; repeat red; sis; auto.
   Qed.
@@ -467,7 +468,7 @@ Module ParserFn (Import D : Defs.T).
     let hr := mkRhsMap_correct gr in
     let cm := mkClosureMap gr     in
     fun (x : nonterminal) (ts : list token) =>
-      let sk0 := (Fr x [] tt [NT x], []) in
+      let sk0 := (Fr [] tt [NT x], []) in
       multistep gr hw rm hr cm sk0 ts NtSet.empty true empty_cache
                 (cache_invar_starts_true rm cm)
                 (push_invar_starts_true _ _)
